So now we can show stuff about aexpr and bexpr why?

code/wp.thy
@@ -2,16 +2,17 @@ theory wp
 imports Main
 begin
 
-type_synonym 'id state = "'id \<Rightarrow> int option"
+type_synonym state = "string \<Rightarrow> int option"
 
-datatype 'id "aexpr" =
+datatype "aexpr" =
     Cst int
-  | Var 'id
-  | Sub "'id aexpr" "'id aexpr"
+  | Var string
+  | Sub aexpr aexpr
+  | Mul aexpr aexpr 
 
 datatype 'ty "behaviour" = Enormal 'ty | Eunbound
 
-inductive eval_aexpr :: "'id aexpr \<Rightarrow> 'id state \<Rightarrow> int behaviour \<Rightarrow> bool" where
+inductive eval_aexpr :: "aexpr \<Rightarrow> state \<Rightarrow> int behaviour \<Rightarrow> bool" where
     eval_cst : "eval_aexpr (Cst n) s (Enormal n)"
   | eval_var : "s x = Some n \<Longrightarrow> eval_aexpr (Var x) s (Enormal n)"
   | eval_var_err : "s x = None \<Longrightarrow> eval_aexpr (Var x) s Eunbound"
@@ -20,32 +21,37 @@ inductive eval_aexpr :: "'id aexpr \<Rightarrow> 'id state \<Rightarrow> int beh
                 eval_aexpr (Sub a1 a2) s (Enormal (n1 - n2))"
   | eval_sub_err1 : "eval_aexpr a1 s Eunbound \<Longrightarrow>
                      eval_aexpr (Sub a1 a2) s Eunbound"
-  | eval_sub_err2 : "eval_aexpr a2 s Eunbound \<Longrightarrow>
+  | eval_sub_err2 : "eval_aexpr a1 s (Enormal n) \<Longrightarrow>
+                     eval_aexpr a2 s Eunbound \<Longrightarrow>
                      eval_aexpr (Sub a1 a2) s Eunbound"
+  | eval_mul : "eval_aexpr a1 s (Enormal n1) \<Longrightarrow>
+                eval_aexpr a2 s (Enormal n2) \<Longrightarrow>
+                eval_aexpr (Mul a1 a2) s (Enormal (n1 * n2))"
+  | eval_mul_err1 : "eval_aexpr a1 s Eunbound \<Longrightarrow>
+                     eval_aexpr (Mul a1 a2) s Eunbound"
+  | eval_mul_err2 : "eval_aexpr a1 s (Enormal n) \<Longrightarrow>
+                     eval_aexpr a2 s Eunbound \<Longrightarrow>
+                     eval_aexpr (Mul a1 a2) s Eunbound"
 
-lemmas [intro] = eval_cst eval_var eval_var_err eval_sub eval_sub_err1 eval_sub_err2
+code_pred eval_aexpr .
 
-primrec aeval :: "'id state \<Rightarrow> 'id aexpr \<Rightarrow> int behaviour" ("_\<lbrakk>_\<rbrakk>a" [999,0] 1000) where
+lemmas [intro] = eval_cst eval_var eval_var_err eval_sub eval_sub_err1 eval_sub_err2 eval_mul eval_mul_err1 eval_mul_err2
+
+primrec aeval :: "state \<Rightarrow> aexpr \<Rightarrow> int behaviour" ("_\<lbrakk>_\<rbrakk>a" [999,0] 1000) where
   "S\<lbrakk>Cst c\<rbrakk>a = Enormal c"
 | "S\<lbrakk>Var x\<rbrakk>a = (case S x of Some n \<Rightarrow> Enormal n | None \<Rightarrow> Eunbound)"
 | "S\<lbrakk>Sub a0 a1\<rbrakk>a = (case (S\<lbrakk> a0 \<rbrakk>a , S\<lbrakk> a1 \<rbrakk>a) of
                            (Enormal n0, Enormal n1) \<Rightarrow> Enormal (n0 - n1)
                            | (_,_) \<Rightarrow> Eunbound)"
+| "S\<lbrakk>Mul a0 a1\<rbrakk>a = (case (S\<lbrakk> a0 \<rbrakk>a , S\<lbrakk> a1 \<rbrakk>a) of
+                           (Enormal n0, Enormal n1) \<Rightarrow> Enormal (n0 * n1)
+                           | (_,_) \<Rightarrow> Eunbound)"
 
 
-
-lemma eval_aexpr_fun : "\<lbrakk> eval_aexpr a s b1; eval_aexpr a s b2 \<rbrakk> \<Longrightarrow> b1 = b2"
-    proof(induction a arbitrary: s b1 b2)
-          case (Cst x)
-       then show ?case by (smt (verit, best) aexpr.distinct(1) aexpr.distinct(3) aexpr.inject(1) eval_aexpr.cases)
-        next
-       case (Var x)
-       then show ?case by (smt (verit) aexpr.distinct(2) aexpr.distinct(6) aexpr.inject(2) eval_aexpr.simps option.discI option.sel)
-        next
-       case (Sub a1 a2)
-       then show ?case by (smt (verit, best) aexpr.distinct(3) aexpr.distinct(5) aexpr.inject(3) behaviour.distinct(1) behaviour.inject eval_aexpr.cases)
-        qed
-
+lemma eval_aexpr_fun : 
+  "\<lbrakk>eval_aexpr a s b1; eval_aexpr a s b2\<rbrakk> \<Longrightarrow> b1 = b2"
+  by (metis Abs_unit_inverse Collect_cong Rep_unit UNIV_def bot_unit_def default_unit_def elem_set
+     eval_single mem_Collect_eq old.unit.exhaust option.inject option.simps(15) singleI_unit sup_bot.monoid_axioms)
 
 lemma eval_aexpr_total :
   shows "eval_aexpr a S Eunbound \<or> (\<exists> n. eval_aexpr a S (Enormal n))"
@@ -58,10 +64,13 @@ lemma eval_aexpr_total :
           next
             case (Sub a1 a2)
             then show ?case by (meson eval_sub eval_sub_err1 eval_sub_err2)
+          next
+            case (Mul a1 a2)
+            then show ?case by (meson eval_mul eval_mul_err1 eval_mul_err2)
           qed
-
+          
 lemma eval_aexpr_equiv: "(S\<lbrakk> a \<rbrakk>a = result) \<Longrightarrow> eval_aexpr a S result"
-  proof(induction a arbitrary: S result)
+proof(induction a arbitrary: result)
           case (Cst x)
        then show ?case by fastforce
         next
@@ -69,10 +78,14 @@ lemma eval_aexpr_equiv: "(S\<lbrakk> a \<rbrakk>a = result) \<Longrightarrow> ev
        then show ?case by (metis aeval.simps(2) eval_var eval_var_err option.split_sel)
         next
        case (Sub a1 a2)
-       then show ?case sorry
+       then show ?case
+         apply(simp)
+         by (smt (verit, del_insts) behaviour.simps(4) behaviour.simps(5)
+             eval_aexpr_fun eval_aexpr_total eval_sub eval_sub_err1 eval_sub_err2)
+        next
+        case (Mul a1 a2)
+        then show ?case
+         apply(simp)
+         by (smt (verit, del_insts) behaviour.simps(4) behaviour.simps(5)
+             eval_aexpr_fun eval_aexpr_total eval_mul eval_mul_err1 eval_mul_err2)
         qed
-
-
-
-(* lemma eval_aexpr_total "eval_aexpr a s Eunbound \<or> (\<exists> n. eval_aexpr a s (Enormal n))"
- *   proof(induction a) *)
